language/move-prover/src/main.rs
@@ -11,7 +11,7 @@ use std::env;
 fn main() -> anyhow::Result<()> {
     let mut options = Options::default();
     let args: Vec<String> = env::args().collect();
-    options.initialize_from_args(&args);
+    options.initialize_from_args(&args)?;
     options.setup_logging();
     let mut error_writer = StandardStream::stderr(ColorChoice::Auto);
     run_move_prover(&mut error_writer, options)
