language/move-prover/src/prelude_template_helpers.rs
@@ -1,0 +1,59 @@
+// Copyright (c) The Libra Core Contributors
+// SPDX-License-Identifier: Apache-2.0
+
+use handlebars::{
+    to_json, BlockContext, Context, Handlebars, Helper, HelperDef, HelperResult, Output,
+    RenderContext, RenderError, Renderable,
+};
+
+#[derive(Clone, Copy)]
+pub struct StratificationHelper {
+    depth: usize,
+}
+
+impl StratificationHelper {
+    pub fn new(depth: usize) -> Self {
+        Self { depth }
+    }
+}
+
+impl HelperDef for StratificationHelper {
+    fn call<'reg: 'rc, 'rc>(
+        &self,
+        h: &Helper<'reg, 'rc>,
+        r: &'reg Handlebars,
+        ctx: &'rc Context,
+        rc: &mut RenderContext<'reg, 'rc>,
+        out: &mut dyn Output,
+    ) -> HelperResult {
+        if !h.params().is_empty() {
+            return Err(RenderError::new("helper cannot have parameters"));
+        }
+        let templ = h
+            .template()
+            .ok_or_else(|| RenderError::new("expected block template"))?;
+        let inverse = h
+            .inverse()
+            .ok_or_else(|| RenderError::new("expected else template"))?;
+
+        for i in 0..self.depth {
+            let this_suffix = if i == 0 {
+                "stratified".to_owned()
+            } else {
+                format!("level{}", i)
+            };
+            let next_suffix = format!("level{}", i + 1);
+            rc.push_block(BlockContext::new());
+            let block = rc.block_mut().expect("block defined");
+            block.set_local_var("@this_suffix".to_owned(), to_json(this_suffix));
+            block.set_local_var("@next_suffix".to_owned(), to_json(next_suffix));
+            block.set_local_var("@this_level".to_owned(), to_json(i));
+            if i == self.depth - 1 {
+                inverse.render(r, ctx, rc, out)?;
+            } else {
+                templ.render(r, ctx, rc, out)?;
+            }
+        }
+        Ok(())
+    }
+}
