language/move-prover/tests/sources/functional/specs-in-fun.move
@@ -1,6 +1,11 @@
 module TestAssertAndAssume {
     // Tests that should verify
 
+    spec module {
+        pragma verify = true;
+    }
+
+
     fun simple1(x: u64, y: u64) {
         if (!(x > y)) abort 1;
         spec {
